src/program_proof/examples/alloc_crash_proof.v
@@ -581,7 +581,7 @@ Lemma prepare_reserved_block_reuse R' E R n n' γ e a Φ Φc:
                                            reserved_block_in_prep γ n' a ∗
                                            □ (R' v -∗ block_cinv γ a) }}
                                    {{ Φc ∗ ▷ block_cinv γ a }}) -∗
-  WPC e @  (LVL (S (S n))); ⊤; E {{ Φ }} {{ Φc }}.
+  WPC e @  (LVL (S n)); ⊤; E {{ Φ }} {{ Φc }}.
 Proof.
   iIntros (??) "Hreserved H".
   iNamed "Hreserved".
@@ -612,7 +612,7 @@ Lemma prepare_reserved_block E1 E2 R n n' γ e a Φ Φc:
    reserved_block_in_prep γ n' a -∗
    WPC e @ LVL n; (E1 ∖ ↑Ncrash); ∅ {{ λ v, (Φc ∧ Φ v) ∗ block_cinv γ a }}
                                    {{ Φc ∗ ▷ block_cinv γ a }}) -∗
-  WPC e @  (LVL (S (S n))); E1; E2 {{ Φ }} {{ Φc }}.
+  WPC e @  (LVL (S n)); E1; E2 {{ Φ }} {{ Φc }}.
 Proof.
   iIntros (???) "Hreserved H".
   iNamed "Hreserved".
